theories/iris_fundamental_helpers.v
@@ -36,7 +36,7 @@ Ltac take_drop_app_rewrite_twice n m :=
 Section fundamental.
   Import DummyHosts. (* placeholder *)
 
-  Context `{!wfuncG Σ, !wtabG Σ, !wmemG Σ, !wmemsizeG Σ, !wglobG Σ, !wframeG Σ, HWP: host_program_logic, !logrel_na_invs Σ}.
+  Context `{!wfuncG Σ, !wtabG Σ, !wtabsizeG Σ, !wmemG Σ, !wmemsizeG Σ, !wglobG Σ, !wframeG Σ, HWP: host_program_logic, !logrel_na_invs Σ}.
   
   (* --------------------------------------------------------------------------------------- *)
   (* ------------------------------ HELPER TACTICS AND LEMMAS ------------------------------ *)
